Port WriteValue

TM/Code/CodeTM.v
@@ -2,7 +2,6 @@ Require Export TM.Prelim TM.TM TM.Code.Code.
 Require Import TM.Combinators.SequentialComposition.
 Require Import TM.Relations.
 Require Import TM.LiftSigmaTau.
-Require Import TM.Basic.Mono TM.Basic.WriteString.
 Require Import TM.Compound.TMTac.
 
 
@@ -358,7 +357,7 @@ Notation "t '≃(' c ')' x" := (tape_contains (cx := c) t x) (at level 70, no as
 
 
 Notation "t ≃[ r1 ] x" := (tape_contains_r t x r1) (at level 70, no associativity, format "t  ≃[ r1 ]  x").
-Notation "t '≃[' c ']' x" := (tape_contains (cx := c) t x) (at level 70, no associativity, only parsing).
+Notation "t '≃[' c ; r1 ']' x" := (tape_contains_r (cx := c) t x r1) (at level 70, no associativity, only parsing).
 
 
 
@@ -476,89 +475,6 @@ End Test_Computes_Gen2.
 
 
 (* TODO *)
-
-(*
-
-(* Write a value to a tape *)
-Section InitTape.
-
-  Section Write_String_Rev.
-    Variable sig : finType.
-
-    (* This should go directly to WriteString.  It is a better definition *)
-
-    Definition WriteStr_Rev_Rel (str:list sig) : Rel (tapes sig 1) (unit * tapes sig 1) :=
-      Mk_R_p (ignoreParam (fun tin tout => right tout = str ++ right tin)).
-
-    (*
-    Section Test.
-      Let t : tape (FinType(EqType(move))) := midtape [N;N;N;N;N] N [N;N;N;N;N].
-      Let str := [R;R;R;R;R;R;N].
-      Compute rev str ++ right t.
-      Compute right (Tape_Write_String L t str).
-      Compute right (Tape_Write_String L t (str ++ [L;R])).
-      Compute Tape_Write_String L t (rev str).
-      Compute Tape_Write_String L (Tape_Write_String L t [L;R]) str.
-      Compute Tape_Write_String L t ([L;R] ++ str).
-    End Test.
-     *)
-
-    Lemma Tape_Write_String_L_cont (str str' : list sig) (t : tape sig) :
-      Tape_Write_String L t (str ++ str') = Tape_Write_String L (Tape_Write_String L t str) str'.
-    Proof. revert t str'. induction str; intros; cbn in *; auto. Qed.
-
-    Lemma Tape_Write_String_L_right' (str : list sig) : forall t : tape sig,
-        right (Tape_Write_String L t str) = List.rev str ++ right t.
-    Proof.
-      induction str; intros; cbn in *; auto.
-      destruct t; cbn; simpl_list; rewrite IHstr; cbn; auto.
-      destruct l; cbn; auto.
-    Qed.
-
-    Lemma Tape_Write_String_L_right (str : list sig) : forall t : tape sig,
-        right (Tape_Write_String L t (List.rev str)) = str ++ right t.
-    Proof. intros. rewrite <- (rev_involutive str) at 2. apply Tape_Write_String_L_right'. Qed.
-
-    Lemma WriteStr_Rev_Sem (str:list sig) :
-      Write_String L tt (List.rev str) ⊨c(4 * |str|) WriteStr_Rev_Rel str.
-    Proof.
-      eapply RealiseIn_monotone.
-      - eapply Write_string_Sem.
-      - simpl_list. omega.
-      - intros tin (()&tout); TMSimp; subst. clear H0. apply Tape_Write_String_L_right.
-    Qed.
-
-  End Write_String_Rev.
-
-
-  Variable sig : finType.
-  Variable X : Type.
-  Hypothesis codX : codeable sig X.
-
-  Definition InitTape_Rel (x : X) : Rel (tapes sig^+ 1) (unit * tapes sig^+ 1) :=
-    Mk_R_p (ignoreParam (fun _ tout => tape_encodes _ tout x)).
-
-  Definition InitTape (x : X) : { M : mTM sig^+ 1 & states M -> unit } :=
-    Write_String L tt (List.rev (inl START :: List.map inr (encode (codeable := codX) x) ++ [inl STOP]));; Move _ R tt;; Move _ R tt.
-
-
-  Lemma InitTape_Sem (x : X) :
-    InitTape x ⊨c(12 + 4 * |encode x|) InitTape_Rel x.
-  Proof.
-    eapply RealiseIn_monotone.
-    - eapply Seq_RealiseIn. eapply WriteStr_Rev_Sem.
-      eapply Seq_RealiseIn; eapply Move_Sem.
-    - cbn. simpl_list. cbn. omega.
-    - intros tin (()&tout). hnf. TMSimp; clear_trivial_eqs; subst.
-      destruct_tapes; cbn in *. subst.
-      destruct h0; cbn in *; inv H; cbn.
-      + simpl_tape. destruct (encode x) eqn:E; cbn; do 2 eexists; split; hnf; cbn; try rewrite E; simpl_list; cbn; eauto.
-      + destruct (encode x) eqn:E; cbn; do 2 eexists; split; hnf; cbn; try rewrite E; simpl_list; cbn; eauto.
-  Qed.
-
-End InitTape.
-
-*)
 
 
 (*
